Benchmark/List/Examples/K.lean
@@ -1,0 +1,129 @@
+import Autoinc.Combinator
+import Autoinc.Data.Seq.Operator
+import Autoinc.Data.Nat.Operator
+import Autoinc.Data.List.Operator
+import Benchmark.Experiment
+import Benchmark.List.Random
+import AssertCmd
+open Experiment
+namespace Example11
+
+open StructProd3
+
+namespace Benchmark
+
+abbrev A := (List Nat) × Nat
+abbrev B := Nat
+abbrev ΔA := ΔProd (ΔList Nat ΔNat) ΔNat
+abbrev ΔB := List ΔNat
+
+abbrev γ₁ := List Nat
+abbrev Env₁ := LazyEagerState γ₁ (Nat × Nat)
+-- TODO: is this the correct type and if so, why? I just satisfied the type checker but have no idea why this works
+def op₁ : Operator A B ΔA ΔB (StateT Env₁ IO) := ΔList.Count.op (LazyEagerStateT γ₁ (Nat × Nat) _) (α := Nat) (Δα := ΔNat) (γ := γ₁)
+
+abbrev γ₂ := Tree Nat
+abbrev Env₂ := LazyEagerState γ₂ (Nat × Nat)
+def op₂ : Operator A B ΔA ΔB (StateT Env₂ IO) := ΔList.Count.op (LazyEagerStateT γ₂ (Nat × Nat) _) (α := Nat) (Δα := ΔNat) (γ := γ₂)
+
+abbrev inputSize := 9000
+abbrev input₁ := List.range inputSize
+abbrev input₂ := inputSize / 3
+abbrev input := (input₁, input₂)
+
+instance : SizeOf A where
+  sizeOf _ := inputSize
+
+def buildCase₁ (id : Nat) (description : String) (genChange : StdGen → Nat → ΔA) (rep:Nat:=100) : Case A B ΔA ΔB Env₁ where
+  op := op₁
+  id := id
+  description := description
+  rep := rep
+  input := input
+  p := 5
+  genChange := genChange
+
+def buildCase₂ (id : Nat) (description : String) (genChange : StdGen → Nat → ΔA) (rep:Nat:=100) : Case A B ΔA ΔB Env₂ where
+  op := op₂
+  id := id
+  description := description
+  rep := rep
+  input := input
+  p := 5
+  genChange := genChange
+
+def buildCases (id : Nat) (description : String) (genChange : StdGen → Nat → ΔA) (rep:Nat:=100) :=
+  let case₁ := buildCase₁ id description genChange rep
+  let case₂ := buildCase₂ id description genChange rep
+  (case₁, case₂)
+
+/-
+Optimal case:
+- Only inserts (no need to update internal list representation)
+-/
+
+def case_1 :=
+  buildCases
+    1
+    "insert elements in the first part of the list"
+    (fun g size => randIns 1 1000 size g |>.1 |> ΔProd._1)
+
+def case_2 :=
+  buildCases
+    2
+    "insert elements in the middle part of the list"
+    (fun g size => randIns 4000 5000 size g |>.1 |> ΔProd._1)
+
+def case_3 :=
+  buildCases
+    3
+    "insert elements in the last part of the list"
+    (fun g size => randIns 8000 9000 size g |>.1 |> ΔProd._1)
+
+
+def case_4 :=
+  buildCases
+    4
+    "delete elements in the first part of the list"
+    (fun g size => randDel 1 1000 size g |>.1 |> ΔProd._1)
+
+def case_5 :=
+  buildCases
+    5
+    "delete elements in the middle part of the list"
+    (fun g size => randDel 4000 5000 size g |>.1 |> ΔProd._1)
+
+def case_6 :=
+  buildCases
+    6
+    "delete elements in the last part of the list"
+    (fun g size => randDel 8000 9000 size g |>.1 |> ΔProd._1)
+
+
+def cases :=
+  [
+    case_1,
+    case_2,
+    case_3,
+    case_4,
+    case_5,
+    case_6,
+    -- case_7,
+    -- case_8,
+    -- case_9,
+    -- case_10,
+    -- case_11,
+    -- case_12
+  ]
+
+def cases₁ := cases.map (·.1)
+def cases₂ := cases.map (·.2)
+
+
+end Benchmark
+
+
+
+
+
+end Example11
