Benchmark/Main.lean
@@ -2,15 +2,19 @@ import Autoinc
 import Benchmark.List.Examples
 import Benchmark.Experiment
 import Benchmark.ExperimentReaderT
+import Benchmark.Sequence
 
 def main : IO Unit := do
-  Case.execAll' Example1.Benchmark.cases (caption:="tail -> tail -> tail -> head")
-  Case.execAll' Example2.Benchmark.cases (caption:="append -> append -> length")
-  ExperimentReaderT.Case.execAll' Example3.Benchmark.cases_1.1 Example3.Benchmark.cases_1.2 (caption:="drop -> take -> all")
-  ExperimentReaderT.Case.execAll' Example3.Benchmark.cases_2.1 Example3.Benchmark.cases_2.2 (caption:="drop -> take -> all")
-  ExperimentReaderT.Case.execAll' Example4.Benchmark.cases_1.1 Example4.Benchmark.cases_1.2   (caption:="drop -> take -> any")
-  ExperimentReaderT.Case.execAll' Example4.Benchmark.cases_2.1 Example4.Benchmark.cases_2.2   (caption:="drop -> take -> any")
-  Case.execAll' Example7.Benchmark.cases (caption:="reverse -> tail -> cons -> reverse -> head")
-  Case.execAll' Example8.Benchmark.cases (caption:="append -> cons -> tail -> reverse -> length")
-  ExperimentReaderT.Case.execAll' Example9.Benchmark.cases_1.1 Example9.Benchmark.cases_1.2 (caption:="drop -> reverse -> drop -> reverse -> all")
-  ExperimentReaderT.Case.execAll' Example9.Benchmark.cases_2.1 Example9.Benchmark.cases_2.2 (caption:="drop -> reverse -> drop -> reverse -> all")
+  -- Case.execAll' Example1.Benchmark.cases (caption:="tail -> tail -> tail -> head")
+  -- Case.execAll' Example2.Benchmark.cases (caption:="append -> append -> length")
+  -- ExperimentReaderT.Case.execAll' Example3.Benchmark.cases_1.1 Example3.Benchmark.cases_1.2 (caption:="drop -> take -> all")
+  -- ExperimentReaderT.Case.execAll' Example3.Benchmark.cases_2.1 Example3.Benchmark.cases_2.2 (caption:="drop -> take -> all")
+  -- ExperimentReaderT.Case.execAll' Example4.Benchmark.cases_1.1 Example4.Benchmark.cases_1.2   (caption:="drop -> take -> any")
+  -- ExperimentReaderT.Case.execAll' Example4.Benchmark.cases_2.1 Example4.Benchmark.cases_2.2   (caption:="drop -> take -> any")
+  -- Case.execAll' Example7.Benchmark.cases (caption:="reverse -> tail -> cons -> reverse -> head")
+  -- Case.execAll' Example8.Benchmark.cases (caption:="append -> cons -> tail -> reverse -> length")
+  -- ExperimentReaderT.Case.execAll' Example9.Benchmark.cases_1.1 Example9.Benchmark.cases_1.2 (caption:="drop -> reverse -> drop -> reverse -> all")
+  -- ExperimentReaderT.Case.execAll' Example9.Benchmark.cases_2.1 Example9.Benchmark.cases_2.2 (caption:="drop -> reverse -> drop -> reverse -> all")
+  -- Case.execAll' Example11.Benchmark.cases₁ (caption := "count with list")
+  -- Case.execAll' Example11.Benchmark.cases₂ (caption := "count with tree")
+  execAll
