Benchmark/Sequence.lean
@@ -1,0 +1,86 @@
+import Benchmark.List.Random
+import Autoinc.SequenceTree
+import Benchmark.Utils
+import Benchmark.Table
+
+def forceSequence [Sequence β γ] (s : γ) : IO Nat := do
+  let mut x := 0
+  let t₁ ← IO.monoNanosNow
+  for _ in Sequence.toList s do
+    x := x + 1
+  let t₂ ← IO.monoNanosNow
+  return t₂ - t₁
+
+-- benchmark patching list with changes vs patching tree with changes
+def benchmark [Sequence β γ] (f : α → γ) (input : α) (rep : Nat := 50) : IO Float := do
+  let mut total : UInt64 := 0
+  for _ in [0:rep] do
+    let start ← IO.monoNanosNow
+    let result := f input
+    let t ← forceSequence result
+    let stop ← IO.monoNanosNow
+    total := total + (stop - start - t).toUInt64
+  return total.toFloat / rep.toFloat
+
+def benchmarkList [Sequence β γ] (f : α → γ) (inputs : List α) (rep : Nat := 50) : IO (List Float) := do
+  let mut totals : List Float := []
+  for input in inputs do
+    let t ← benchmark f input rep
+    totals := t :: totals
+  return totals.reverse
+
+def inputSize := 10000
+def input := List.range inputSize
+def changeSize := 5.0 -- %
+
+def exec [Sequence β γ] (name : String) (f : ΔList Nat ΔNat → γ) (inputs : List (String × ΔList Nat ΔNat)) : IO Unit := do
+  let unnamedInputs := inputs.map (·.2)
+  let inputNames := inputs.map (·.1)
+  IO.println name
+  IO.println "------"
+  let results ← benchmarkList f unnamedInputs
+  let namedResults := inputNames.zip results
+  for (inputName, t) in namedResults do
+    IO.println s!"{inputName} | {t.trunc 3}ns"
+  IO.println "------"
+
+def at_p (p : Float) (size : Nat) : Nat :=
+  p * size.toFloat |>.toUInt64 |>.toNat
+
+def execAll : IO Unit := do
+  let list := Sequence.fromList (γ := List Nat) input
+  let tree := Sequence.fromList (γ := Tree Nat) input
+  let size := (changeSize / 100.0) * inputSize.toFloat |> (·.toUInt64.toNat)
+  let gen ← IO.stdGenRef.get
+  let inputs := [
+    ("Insertion at the start of the list", randIns (at_p 0 inputSize) (at_p 0.1 inputSize) size gen |>.1),
+    ("Insertion in the middle of the list", randIns (at_p 0.45 inputSize) (at_p 0.55 inputSize) size gen |>.1),
+    ("Insertion at the end of the list", randIns (at_p 0.8 inputSize) (at_p 0.9 inputSize) size gen |>.1),
+
+    ("Deletion at the start of the list", randDel (at_p 0 inputSize) (at_p 0.1 inputSize) size gen |>.1),
+    ("Deletion in the middle of the list", randDel (at_p 0.45 inputSize) (at_p 0.55 inputSize) size gen |>.1),
+    ("Deletion at the end of the list", randDel (at_p 0.8 inputSize) (at_p 0.9 inputSize) size gen |>.1),
+
+    ("Update at the start of the list", randUpd (at_p 0 inputSize) (at_p 0.1 inputSize) size gen |>.1),
+    ("Update in the middle of the list", randUpd (at_p 0.45 inputSize) (at_p 0.55 inputSize) size gen |>.1),
+    ("Update at the end of the list", randUpd (at_p 0.8 inputSize) (at_p 0.9 inputSize) size gen |>.1),
+  ]
+
+  exec "List" (list ⨁ ·) inputs
+  exec "Tree" (tree ⨁ ·) inputs
+
+  let inputNames := inputs.map (·.1)
+  let inputValues := inputs.map (·.2)
+  let listTimes ← benchmarkList (list ⨁ ·) inputValues
+  let treeTimes ← benchmarkList (tree ⨁ ·) inputValues
+  let speedups := listTimes.zip treeTimes |>.map (fun (t₁, t₂) => t₁ / t₂)
+
+  let headers := ["Description", "List", "Tree", "Speedup (List → Tree)"]
+  let rows :=
+    inputNames
+    |>.zip (listTimes.map (·.trunc ++ "ns"))
+    |>.zip (treeTimes.map (·.trunc ++ "ns"))
+    |>.zip (speedups.map (·.trunc))
+    |>.map (fun (((n, l), t), s) => [n, l, t, s])
+
+  printTable headers rows
